Utilities/Index.thy
@@ -8,6 +8,9 @@ definition incr :: "nat \<Rightarrow> nat \<Rightarrow> nat" where
 definition decr :: "nat \<Rightarrow> nat \<Rightarrow> nat" where
   "decr x y = (if x < y then y - 1 else y)"
 
+definition var_reduce :: "nat \<Rightarrow> nat set \<Rightarrow> nat set" where
+  "var_reduce x xs = decr x ` (xs - {x})"
+
 lemma [simp]: "lookup y as = Some a \<Longrightarrow> x \<le> length as \<Longrightarrow> 
     lookup (incr x y) (insert_at x a' as) = Some a"
   by (simp add: incr_def)
@@ -15,6 +18,65 @@ lemma [simp]: "lookup y as = Some a \<Longrightarrow> x \<le> length as \<Longri
 lemma [simp]: "lookup y (insert_at x a' as) = Some a \<Longrightarrow> x \<le> length as \<Longrightarrow> 
     lookup x' as = Some a' \<Longrightarrow> x \<noteq> y \<Longrightarrow> lookup (decr x y) as = Some a"
   by (cases y) (auto simp add: decr_def)
+
+lemma [simp]: "incr 0 x = Suc x"
+  by (simp add: incr_def)
+
+lemma [simp]: "incr y x \<noteq> y"
+  by (simp add: incr_def)
+
+lemma [simp]: "decr y (incr y x) = x"
+  by (simp add: incr_def decr_def)
+
+lemma [simp]: "x \<noteq> y \<Longrightarrow> incr y (decr y x) = x"
+  by (auto simp add: incr_def decr_def)
+
+lemma [simp]: "y \<noteq> x \<Longrightarrow> decr (Suc y) (incr y x) = x"
+  by (simp add: incr_def decr_def)
+
+lemma [simp]: "y \<le> x \<Longrightarrow> incr y (incr x z) = incr (Suc x) (incr y z)"
+  by (simp add: incr_def)
+
+lemma [simp]: "y \<le> x \<Longrightarrow> y \<noteq> z \<Longrightarrow> decr y (incr (Suc x) z) = incr x (decr y z)"
+  by (auto simp add: incr_def decr_def)
+
+lemma [simp]: "y \<le> x \<Longrightarrow> incr y (decr x z) = decr (Suc x) (incr y z)"
+  by (auto simp add: incr_def decr_def)
+
+lemma [simp]: "y \<notin> xs \<Longrightarrow> (x \<in> decr y ` xs) = (incr y x \<in> xs)"
+  proof rule
+    assume "x \<in> decr y ` xs"
+    then obtain x' where X: "x' \<in> xs \<and> x = decr y x'" by auto
+    moreover assume "y \<notin> xs"
+    moreover with X have "y \<noteq> x'" by auto
+    ultimately show "incr y x \<in> xs" by simp
+  next
+    assume "incr y x \<in> xs"
+    moreover hence "x = decr y (incr y x)" by simp
+    ultimately show "x \<in> decr y ` xs" by blast
+  qed
+
+lemma [simp]: "(x \<in> var_reduce y xs) = (incr y x \<in> xs)"
+  by (simp add: var_reduce_def)
+
+lemma [simp]: "(x \<in> incr y ` xs) = (if x = y then False else decr y x \<in> xs)"
+  proof -
+    have "(x \<in> (\<lambda>z. incr y z) ` xs) = (if x = y then False else decr y x \<in> xs)" 
+      by (cases x) (auto simp add: incr_def decr_def)
+    thus "(x \<in> incr y ` xs) = (if x = y then False else decr y x \<in> xs)" by simp
+  qed
+
+lemma [simp]: "y \<le> x \<Longrightarrow> var_reduce y (incr (Suc x) ` xs) = incr x ` var_reduce y xs"
+  by (auto split: if_splits) (auto simp add: incr_def)
+
+lemma [simp]: "y \<le> x \<Longrightarrow> var_reduce y (insert (Suc x) xs) = insert x (var_reduce y xs)"
+  by (auto simp add: incr_def split: if_splits)
+
+lemma [simp]: "y \<le> x \<Longrightarrow> var_reduce y (var_reduce (Suc x) xs) = var_reduce x (var_reduce y xs)"
+  by auto
+
+lemma [simp]: "var_reduce 0 xs \<inter> (op +) y ` ys = {} \<Longrightarrow> xs \<inter> (op +) (Suc y) ` ys = {}"
+  by (auto simp add: var_reduce_def)
 
 lemma [simp]: "(x::nat) \<ge> y \<Longrightarrow> \<exists>z. x = y + z"
   proof (induction x arbitrary: y)
